### 1.26f
$$
\begin{gather*}
\frac{x}{x+2} - \frac{3x+1}{3x} = \\
\frac{3x^2}{3x(x+2)}-\frac{(3x+1)(x+2)}{3x(x+2)} = \\
\frac{3x^2 - 3x^2 - 6x - x -2}{3x^2+6x} = \\
\frac{-7x-2}{3x(x+2)}
\\\\
x \in \mathbb{R} - \{0, -2\}
\end{gather*}
$$
### 1.31 b
$$
\begin{gather*}
\frac{1}{x-2}-\frac{1}{x} - \frac{1}{x^2-2x} = 
\\
\frac{x}{x(x-2)} - \frac{x-2}{x(x-2)} - \frac{1}{x(x-2)} = 
\\
\frac{x-x+2-1}{x(x-2)} = 
\\
\frac{1}{x(x-2)}
\\\\
x \in \mathbb{R} - \{0, 2\}
\end{gather*}
$$
### 1.36 a
$$
\begin{align*}
\frac{x^2-1}{x^2+x-6} \times \frac{x^2+7x+12}{x^2+x-2} = 
\\
\Delta = 1 + 24 &= 25 & x&=\frac{-1\pm5}{2} \\
x_1&=-3 & x_2= 2
\\
\frac{(x-1)(x+1)}{(x+3)(x-2)} \times \frac{}{}
\end{align*}
$$
# Mnożenie i dzielenie ułamków algebraicznych
### 1.33e
$$
\begin{align*}
\frac{x-1}{3} \times \frac{4x}{x^2-x} = 
\\
\frac{4x(x-1)}{3(x^2-x)} = \frac{4x(x-1)}{3x(x-1)} = \frac{4}{3}
\\\\
x \in \mathbb{R} - \{1, 0\}
\end{align*}
$$
### 1.33f
$$
\begin{align*}
\frac{3x-6}{x^2-4} \times \frac{5}{7x} =
\\
\frac{15(x-2)}{7x(x-2)(x+2)} = 
\\
\frac{15}{7x(x+2)}
\\\\
x \in \mathbb{R} - \{0, 2, -2\}
\end{align*}
$$
### 1.34c
$$
\begin{align*}
\frac{x^2-1}{x^2-81} \times \frac{x-9}{x+1} =
\\
\frac{(x-1)(x+1)}{(x-9)(x+9)} \times \frac{x-9}{x+1} =
\\
\frac{x-1}{x+9}
\\\\
x \in \mathbb{R}- \{9, -9\}
\end{align*}
$$
### 1.34e
$$
\begin{align*}
\frac{x^3+8}{3x^2-3} \times \frac{6x+6}{x^2-2x+4} =
\\
\frac{(x+2)(x^2 - 2x +4)}{3(x-1)(x+1)} \times \frac{6(x+1)}{x^2-2x+4} = 
\\
\frac{6(x+2)}{3(x-1)} = 
\frac{2x+4}{x-1}
\\\\
x \in \mathbb{R} - \{1, -1\}
\end{align*}
$$
### 1.35b
$$
\begin{align*}
\frac{4x^3-8x^2}{16x^2-64} \times \frac{4x+8}{x^2} = 
\\
\frac{4x^2(x-2)}{(4x-8)(4x+8)} \times \frac{4x+8}{x^2} = 
\\
\frac{4(x-2)}{4x-8} = 1
\\\\
x \in \mathbb{R} - \{2, -2\}
\end{align*}
$$


**HOMEWORK: 1.36d,f; 1.37c,**

### 1.36d
$$
\begin{gather*}
\frac{5x^{2}+7x+2}{x^{2}+2x+1} \times \frac{3x^{2}+2x-1}{25x^{2}-4} = \\
\frac{5x^{2}+7x+2}{(x+1)^2} \times \frac{3x^2+2x-1}{(5x-2)(5x+2)} \\
\\\\
\Delta_{1} = 49 - 40 = 9 \\
x = \frac{-7 \pm 3}{10} \\
x_{1} = \frac{-7 + 3}{10} = -\frac{2}{5} \\
x_{2} = \frac{-7 - 3}{10} = -1
\\\\
\frac{5(x+1)\left( x+\frac{2}{5} \right)}{(x+1)^2} \times \frac{3x^2+2x-1}{(5x-2)(5x+2)}
\\\\
\Delta_{2} = 4 + 12 = 16 \\
x = \frac{-2 \pm 4}{6} \\
x_{1} = -1 \\
x_{2} = \frac{1}{3}
\\\\
\frac{(x+1)(5x+2)}{(x+1)^2} \times \frac{3(x+1)\left( x-\frac{1}{3} \right)}{(5x-2)(5x+2)} = \\
\frac{3x-1}{5x-2}
\\ \\
x \in \mathbb{R} - \left\{ -1, \pm \frac{2}{5} \right\}
\end{gather*}

$$
### 1.36f
$$
\begin{gather*}
\frac{2x^2+9x-5}{5x^2+3x-2} \times \frac{x^2+4x+3}{2x^2+5x-3} = \\
\Delta_{1} = 81 + 40 = 121 \\
x = \frac{-9 \pm 11}{4} \\
x_{1} = -5 \ x_{2} = \frac{1}{2} \\
\\ \\
\Delta_{2} = 9 + 40 = 49 \\
x = \frac{-3 \pm 7}{10} \\
x_{1} = -1 \ x_{2} = \frac{2}{5}
\\ \\
\frac{2(x+5)\left( x-\frac{1}{2} \right)}{5(x+1)\left( x-\frac{2}{5} \right)} \times \frac{x^2+4x+3}{2x^2+5x-3} =
\\ \\
\Delta_{4} = 16 - 12 = 4 \\
x = \frac{-4 \pm 2}{2} \\
x_{1} = -3 \ x_{2} = -1
\\ \\
\Delta_{4} = 25 + 24 = 49 \\
x = \frac{-5 \pm 7}{4} \\
x_{1} = \frac{1}{2} \ x_{2} = -3
\\ \\
\frac{2(x+5)\left( x-\frac{1}{2} \right)}{5(x+1)\left( x-\frac{2}{5} \right)} \times \frac{(x+3)(x+1)}{2\left( x-\frac{1}{2} \right)(x+3)} = \\
\frac{x+5}{5\left( x-\frac{2}{5} \right)}
\\ \\
x \in \mathbb{R} - \left\{ -1, \frac{2}{5}, \frac{1}{2}, -3 \right\}
\end{gather*}
$$
### 1.37 c
$$
\begin{gather*}

\frac{2x^3-14x^2-8x+56}{2x^2-18} \times \frac{3x^2+7x-6}{x^2-9x+14}\\ \\

  \begin{array}{c|cccc}
        & 2 & -14 & -8 & 56 \\
       2&  &  4 &  -20 &  -56   \\ \hline
        & 2 & -10 & -28 &|0&
\end{array} \\ \\
\frac{(x-2)(2x^2-10x-28)}{2(x-3)(x+3)} \times \frac{3x^2+7x-6}{x^2-9x+14} \\ \\
\Delta_{1} = 49 + 72 = 121 \\
x = \frac{-7 \pm 11}{6} \\
x_{1} = -3 \ x_{2} = \frac{2}{3}
\\ \\
\Delta_{2} = 81 - 56 = 25
x = \frac{9 \pm 5}{2} \\
x_{1} = 7 \ x_{2} = 2 \\ \\

\frac{(x-2)(2x^2-10x-28)}{2(x-3)(x+3)} \times \frac{3(x+3)\left( x-\frac{2}{3} \right)}{(x-7)(x-2)} \\ \\
\Delta_{3} = 100 + 224 = 324 \\
x = \frac{10 \pm 18}{4} \\
x_{1} = 14 \ x_{2} = -2 \\ \\
\frac{(x-2)2(x-14)(x+2)}{2(x-3)(x+3)} \times \frac{3(x+3)\left( x-\frac{2}{3} \right)}{(x-7)(x-2)} \\ \\
\end{gather*}

$$