### 1.39 e
$$
\begin{gathered}

\frac{x^2-2x+1}{4x^2+2x+1} : \frac{3x^2-3}{8x^3-1} = \\
\frac{(x-1)^2}{4x^2+2x+1} \times \frac{(2x-1)(4x^2+2x+1)}{3(x-1)(x+1)} = \\
\frac{(x-1)(2x-1)}{3(x+1)} = \frac{2x^2-x+1}{3x+3} \\ \\
x \in \mathbb{R} - \left\{ \frac{1}{2},1,-1 \right\}
\end{gathered}
$$

### 1.40 d
$$
\begin{gathered}
\frac{2x^2+5x-3}{10x-20} : \frac{4x^2-1}{3x-6} = \\
\Delta = 25+24 = 49 \\
x_{1} = \frac{-5+7}{4} = \frac{1}{2} \
x_{2} = \frac{-5-7}{4} = -3 
\\ \\
\frac{2(x+3)\left( x-\frac{1}{2} \right)}{10(x-2)} \times \frac{3(x-2)}{(2x-1)(2x+1)} = \\
\frac{3x+9}{20x+10} \\ \\
x \in \mathbb{R} - \left\{ 2, \frac{1}{2}, -\frac{1}{2} \right\}

\end{gathered}
$$

### 1.41 a
$$
\begin{gathered}
\frac{x^3+8x^2-x-8}{x^2+9x+8} : \frac{2x^2-2}{x+3} = \\
\frac{x^2(x+8)-1(x+8)}{x^2+1x+8x+8} \times \frac{x+3}{2(x+2)(x-2)} = \\
\frac{(x+1)(x-1)(x+8)}{(x+8)(x+1)} \times \frac{(x+3)}{2(x+2)(x-2)} = \\
\frac{x+3}{2x+2} \\ \\
x \in \mathbb{R} - \{-8, -1, \pm{2} \}
\end{gathered}
$$

# Działania na ułamkach algebraicznych

### 1.42 d
$$
\begin{gathered}
\frac{1+\frac{1}{x+1}}{3-\frac{2}{x+1}} = \frac{\frac{x+2}{x+1}}{\frac{3x+1}{x+1}} = \\
\frac{x+2}{3x+1} \\ \\
x \in \mathbb{R} - \left\{ -1, -\frac{1}{3} \right\}
\end{gathered}
$$

### 1.43 f
$$
\begin{gathered}
\Huge
\frac{\frac{2x}{x-1} - \frac{x}{x+2}}{\frac{x+5}{1-x^2}} = \frac{\frac{2x(x+2)-x(x-1)}{(x-1)(x+2)}}{\frac{x+5}{(1-x)(x+1)}} = \\
\Huge
\frac{\frac{2x^2+4x-x^2+x}{(x-1)(x+2)}}{\frac{x+5}{(1-x)(x+1)}} = 
\frac{\frac{x(x+5)}{(x-1)(x+2)}}{\frac{x+5}{(1-x)(x+1)}} = \\
\Huge
\frac{\frac{x}{x+2}}{\frac{1}{x+1}} = - \frac{x^2 + x}{x+2} \\ \\
x \in \mathbb{R} - \{1, -1, -2,-5\}

\end{gathered}
$$

### 1.44 f
$$
\begin{gathered}
\left( \frac{1}{2} + \frac{1}{2a^3} \right) : \left( a - 1 + \frac{1}{a} \right) = \left( \frac{a^3+1}{2a^3} \right) : \left( \frac{a^2}{a} - \frac{a}{a} + \frac{1}{a} \right) = \\
\left( \frac{(a+1)(a^2-a+1)}{2a^3} \right):\left( \frac{a^2-a+1}{a} \right) = \\
\frac{(a+1)(a^2-a+1)}{2a^3} \times \frac{a}{a^2-a+1} = \\
\frac{a+1}{2a^2} \\ \\
a \in \mathbb{R} - \{0\}
\end{gathered}
$$

HOMEWORK: 1.52; 1.54; 1.57a

### 1.52
$$
\begin{gathered}
a \in \mathbb{R} - \{-2, 0\}
\\ \\
\left( \frac{a^2}{8} + { \frac{1}{a}} \right) :\left( \frac{a}{4}-\frac{1}{2} +\frac{1}{a} \right): \frac{(a-2)^2 + 8a}{1 + \frac{2}{a}} = \frac{1}{2a} \\
\frac{a^3 + 8}{8a} : \left( \frac{a^2}{4a} -  \frac{2a}{4a} + \frac{4}{4a}\right) : \frac{(a-2)^2 + 8a}{1 + \frac{2}{a}} = \frac{1}{2a} \\
\frac{(a+2)(a^2-2a+4)}{8a} \times \frac{4a}{(a^2-2a+4)} \times \frac{1+\frac{2}{a}}{a^2+4a+4} = \\
\frac{a+2}{2} \times \frac{1+\frac{2}{a}}{(a+2)^2} \times \frac{a}{a} = \frac{a\left( 1+\frac{2}{a} \right)}{2(a+2)a} = \frac{1}{2a}
\\ \\
\text{koniec dowodu}
\end{gathered}
$$

### 1.54
$$
\begin{gathered}
b \ne -\frac{3a}{2}
\\ 
\begin{cases}
\frac{b}{3a+2b} = \frac{1}{5} \\ \\
\frac{4a+5b}{11a-2b} = 1
\end{cases} \\
\begin{cases}
5b = 3a+2b \\
4a+5b = 11a-2b
\end{cases}
\\
\\
3b = 3a \implies b=a \\

\frac{4a+5a}{11a-2a} = \frac{9a}{9a} = 1 \\ 
\text{koniec dowodu}
\end{gathered}
$$

### 1.57 a
$$
\begin{gathered}
\left( \frac{1}{x+1} + x\right)\times\left( \frac{x}{x-1}-1 \right) - \left( \frac{1}{x+1}+1 \right)\times\left( \frac{1}{x-1} -x \right) = \\
\frac{x^2+x+1}{x+1} \times \frac{x-x+1}{x-1} -\frac{1+x+1}{x+1}\times \frac{1-x^2+x}{x-1} = \\ \\
\frac{x^2+x+1}{(x+1)(x-1)} - \frac{(2+x)(1-x^2+x)}{(x+1)(x-1)} = \\ \\
\frac{x^2+x+1}{(x+1)(x-1)} - \frac{2 - 2x^2 +2x +x -x^3 +x^2}{(x+1)(x-1)} = \\ \\
\frac{x^2+x+1}{(x+1)(x-1)} - \frac{2 -x^2 +3x -x^3}{(x+1)(x-1)} = \\ \\
\frac{x^2+x+1 - 2 +x^2 -3x + x^3}{(x+1)(x-1)} = \\
\frac{2x^2 - 1 -2x + x^3}{(x+1)(x-1)} = \\
\frac{2x^2-2x + x^3- 1}{(x+1)(x-1)} = \\
\frac{2x(x-1) + (x-1)(x^2 +x +1)}{(x+1)(x-1)} = \\
\frac{(x-1)(x^2 +1 + 3x)}{(x+1)(x-1)} = \\ \\
\frac{x^2 + 3x +1 }{(x+1)}  \\ \\
x \in \mathbb{R} - \{-1, 1\}
\end{gathered}
$$