# Równania wymierne
Równaie postaci $\frac{W(x)}{P(x)}$ = 0 nazywami równaniem wymiernym przy zcym W(x) i P(x) są wielomianami i P(x) nie jest wielomianem zerowym
$$
\frac{W(x)}{P(x)} = 0 <=> W(x) = 0 ∧ P(x) \ne 0
$$

### 1.64f
$$
\begin{gathered}
\frac{(x-1)(x+2)(x+5)}{x^2+4x-5} = 0 \\
x^2+4x-5 \ne 0 \\
\Delta = 16 + 20 \\
x = \frac{-4 \pm 6}{2} \\
x_{1} = -5 \ x_{2} = 1 \\
x \in \mathbb{R} - \{-5, 1\} \\ \\
x = -2
\end{gathered}
$$ 

### 1.65 a
$$
\begin{gathered}
\frac{(x^3-27)(x^2-16)}{6x-18} = 0 \\
6x-18 \ne 0 \ x\ne 3 \\
x \in \{\pm 4\}
\end{gathered}
$$

### 1.65 f
$$
\begin{gathered}
\frac{(2x^2 + 4x)(3-x)}{x^3-4x^2} = 0 \\
x^2(x-4) \ne 0 \ x\ne 0 \wedge x\ne 4 \\
(2x(x+2))(3-x) = 0 \\
x \in \{3, -2\} 
\end{gathered}
$$

### 1.66 a
$$
\begin{gathered}
\frac{x^3-4x^2+3}{x-1} = 0 \ x \ne 1 \\
x^3-4x^2+3 = 0 \\ \\

\begin{array}{c|cccc}
        & 1 & -4 & 0 & 3 \\
       1  &   &  1 &  -3   \\ \hline
        & 1 & -3 & -3 &|0&
\end{array} \\ \\
(x-1)(x^2-3x-3)= 0 \\
\Delta = 9 +12 = 21 \\
x = \frac{3 \pm \sqrt{ 21 }}{2} \\
x \in \left\{ \frac{3+\sqrt{ 21 }}{2}, \frac{3 - \sqrt{ 21 }}{2} \right\}

\end{gathered}
$$

### 1.67 f
$$
\begin{gathered}
\frac{x+1}{x+2} = \frac{x+2}{x-3} \\
(x+1)(x-3) = (x+2)^2 \\
x^2 -3x +x -3 = x^2+4x +4\\
x^2-2x-3 = x^2+4x+4\\
-6x = 7 \\
x = -\frac{7}{6} \\
x \in \mathbb{R} - \{-2, 3\}
\end{gathered}
$$

### 1.68e
$$
\begin{gathered}
\frac{x}{2x-3} + \frac{1}{3-2x} = 2x-2 \\
\frac{x-1}{3-2x} = \frac{2(x-2)(3-2x)}{3-2x} \\
x-1 = 4x^2-6x-4x+6 \\
x-1 = 4x^2-10x+6 \\
4x^2-11x+7 = 0 \\
\Delta = 121 - 112 = 9 \\
x = \frac{11 \pm 3}{8} \\
x_{1} = \frac{7}{4} \ x_{2} = 1 \\

\end{gathered}
$$

**HOMEWORK : 1.69; 1.70**
### 1.69 
a)
$$
\begin{gathered}
\frac{4}{3x+2} - \frac{5}{x-2} = 0 \\
x \in \mathbb{R} -\left\{ 2, -\frac{2}{3} \right\} \\
\frac{4x-8-15x+10}{(3x+2)(x-2)} = 0 \\
-11x-2 = 0
x = -1 \frac{7}{11}
\end{gathered}
$$
b)
$$
\begin{gathered}
\frac{4}{x} - 1 = \frac{1}{x-1} \\ 
x \in \mathbb{R} - \{0,1\} \\
4(x-1)-x(x-1) = x \\
-x^2+4x-4 = 0\\
(x-2)^2 = 0 \\
x =2
\end{gathered}
$$
c)
$$
\begin{gathered}
\frac{1}{x+2} - \frac{2}{x-1} = 1 \\
x \in \mathbb{R} - \{-2,1\} \\
x-1-2(x+2) = (x+2)(x-1) \\
x-1-2x-4=x^2-x+2x-2 \\
\Delta = 4 -12 = -8 < 0 \\ x \in \emptyset
\end{gathered}
$$
d)
$$
\begin{gathered}
\frac{2}{x-3} + \frac{4x}{x+2} = \frac{1}{3} \\
x \in \mathbb{R} - \{3,-1\} \\
6(x+2) + 12x(x-3) = (x-3)(x+2) \\
6x + 12 + 12x^2-36x = x^2+2x-3x-6 \\
11x^2-29x+18 = 0\\
\Delta = 841-792 = 49
x = \frac{29 \pm 7}{22} \\
x_{1} = \frac{18}{11} \ x_{2} = 1
x \in \left\{ 1, \frac{18}{11} \right\}
\end{gathered}
$$
e)
$$
\begin{gathered}
\frac{1}{2-x}+\frac{4}{x^3-8} = 0 \\
x \in \mathbb{R} - \{2\} \\
-\frac{1}{x-2} + \frac{4}{(x-2)(x^2+2x+4)} = 0 \\
-x^2-2x-4+4 = 0 \\
-x(x+2) = 0 \\
x = -2 \vee x=0
\end{gathered}
$$
f)
$$
\begin{gathered}
\frac{4x^2}{x^3+27} = \frac{1}{9-3x+x^2} \\
x \ne -3 \\
\frac{4x^2}{(x+3)(x^{2}-3x+9)} = \frac{1}{9-3x+x^2} \\
4x^2-x-3 = 0 \\
\Delta = 1 + 48 = 49 \\
x = \frac{1 \pm 7}{8} \\
x_{1} = -\frac{3}{4} \ x_{2} = 1 \\
x \in \left\{ -\frac{3}{4}, 1 \right\}
\end{gathered}
$$

### 1.70
a)
$$
\begin{gathered}
\frac{x+1}{x+2} - \frac{2x}{x+3} = -\frac{1}{5} \\
x \notin \{-3, -2\} \\
5(x+1)(x+3)-10x(x+2) = -(x+2)(x+3) \\
5(x^2+4x+3) - 10x^2 - 20x = -(x^2+5x+6) \\
-4x^2+5x+21 = 0 \\
\Delta = 25 + 336 = 361 \\
x = \frac{-5 \pm 19}{-8} \\
x_{1} = -\frac{7}{4} \ x_{2} = 3 \\
x \in \left\{ -\frac{7}{4}, 3 \right\}
\end{gathered}
$$
b)
$$
\begin{gathered}
\frac{2x}{x-1} - \frac{x}{x+2} = \frac{2x-2}{x^2+x-2} \\
x^2+x-2 \ne 0 \ \ \ \ x^2-x+2x-2 = (x-1)(x+2) \\
x \notin \{-2, 1\} \\
2x(x+2) - x(x-1) = 2x-2 \\
2x^2+4x-x^2+x=2x-2 \\
x^2+3x+2 = 0 \\
\Delta = 9-8 = 1 \\
x = \frac{-3 \pm 1}{2} \\
x_{1} = -1 \ x_{2} = -2 \\
x = -1
\end{gathered}
$$
c)
$$
\begin{gathered}
\frac{x-2}{x+1}-\frac{x+1}{3-x} = \frac{x^2+x+12}{x^2-2x-3} \\
x^2-2x-3 \ne 0 \\
x^2+x-3x-3 = x(x+1)-3(x+1) = (x-3)(x+1) \\
x \notin \{-1,3\} \\
(x-2)(x-3) + (x+1)^2 = x^2 + x +12 \\
x^2 - 5x +6 + x^2 + 2x + 1 = x^2 + x + 12 \\
x^2-4x-5 = 0 \\
\Delta = 16+20 = 36 \\
x = \frac{4 \pm 6}{2} \\
x_{1} = -1 \ x_{2} = 5 \\
x = 5
\end{gathered}
$$
d)
$$
\begin{gathered}
\frac{x}{4-x} + \frac{2}{x+4} = \frac{2x+4}{(4-x)(4+x)} \\
x \notin \{\pm 4\} \\
x(x+4) + 2(4-x) = 2x+4 \\ 
4x+x^2+8-2x=2x+4 \\
x^2 = -4 \\
x \in \emptyset
\end{gathered}
$$
e)
$$
\begin{gathered}
\frac{x^2+5x+4}{x^3+3x^2+3x+1} - \frac{2}{(x+1)^2} = 0 \\ 
x \ne -1 \\
\frac{x^2+x+4x+4}{(x+1)^3} - \frac{2}{(x+1)^2} = 0 \\
\frac{(x+4)(x+1)}{(x+1)^3} - \frac{2}{(x+1)^2} = 0\\
x+2 = 0 \\
x= -2
\end{gathered}
$$
f)
$$
\begin{gathered}
\frac{2x^3+x^2}{(4x-2)(4x+2)} = \frac{2}{2x-1} \\
\frac{x^2(2x+1)}{4(2x-1)(2x+1)} = \frac{2}{2x-1} \\
x \notin \left\{ \pm \frac{1}{2} \right\} \\
\frac{x^2(2x+1)-8(2x+1)}{4(2x-1)(2x+1)} = \\
\frac{(x^2-8)(2x+1)}{4(2x-1)(2x+1)} = 0\\
x \in \{\pm 2\sqrt{2} \}
\end{gathered}
$$