### 1.71 e
$$
\begin{gathered}
\frac{3}{x} - \frac{4}{x^2-4x+4} = \frac{1}{x^2-2x} \\
x \notin \{0 ,2\} \\
3(x-2)^2-4x-(x-2)^2 = 0 \\
3x^2-12x+12 -4x-x^2-4x+4 = 0 \\
3x^2-17x+14 = 0 \\
\Delta = 289 - 168 = 121 \\
x = \frac{17 \pm 11}{6} \\
x_{1} = -1 \ x_{2} = 4 \frac{2}{3}\\
x \in \left\{ 4 \frac{2}{3} , 1 \right\}
\end{gathered}
$$
### 1.72 d
$$
\begin{gathered}
\frac{5}{x^2-x-x} + \frac{x}{x^2+4x+3} - \frac{2x}{x^2+x-6} = \frac{9}{x^3+2x^2-5x-6} \\
x^3+2x^2-5x-6 = 0 \\
x^3 +x^2 + x^2 - 6x -6 + x = x^2(x+1) - 6(x+1) + x(x+1) = \\
(x^2+x-6)(x+1) \\ 
\Delta_{1} = 1 + 24 = 25 \\
x = \frac{1 \pm 5}{2} \\
x_{1} = 3 \ x_{2} = -2 \\
(x^2+x-6)(x+1) = (x+1)(x-3)(x+2) \\ \\
x^2-x-x \ne 0 \\
\Delta = 9 \\
x_{1} = -1 \ x_{2} = 2 \\
\\
x^2+4x+3 \ne 0 \\
\Delta = 4 \\
x_{1} = -3 \ x_{2} = -1 \\ \\
x^2+x-6 \ne 0 \\
\Delta - 5 \\
x_{1} = -3 \ x_{2} = 2 \\

\frac{5}{(x-2)(x+1)} + \frac{x}{(x+3)(x+1)} + \frac{2x}{(x+3)(x-2)} = \frac{9}{(x+1)(x+3)(x-2)} \\
5x+15+x^2-2x+2x^2-2x-9 = 0 \\
-x^2 + x +6 = 0 \\
\Delta = 1+25 = 25 \\
x = \frac{-1 \pm 5}{-2} \\
x_{1} = 3 \ x_{2} = -2 \\
x \notin \{2, -1, -3\} \\ \\
x \in \{-2,3\}


\end{gathered}
$$


# Równanie wymierne z wartością bezwzględną i z parametrem

### 1.76 (interesting)
$$
\begin{gathered}
\frac{(x-m)(x+2m)}{x^2-4} = 0 \\
x \in \mathbb{R} - \{\pm 2\} \\ \\
1)\ x-m = x-2 \\
m = 2 \\
\\ 
2)x+2m = x-2 \\
m=-1
\\ \\
3) x-m = x+2\\
m =-2 \\ \\
4) x+2m = x+2 \\
m=1
\\ \\
5) m = 0 \\
x^2 = 0 \\ \\
m \in \{-2,-1,0,1,2\}
\end{gathered}
$$


**HOMEWORK**: 1.77; 178
### 1.77 (interesting)
$$
\begin{gathered}
\frac{m+2}{x+3} - \frac{x-1}{4} = 0 \\
\frac{4m+8-(x-1)(x+3)}{4x+12} = 0 \\
x \ne -3 \\ \\
4m+8-(x-1)(x+3) = 0 \\
4m+8-x^2-3x+x+3 = 0 \\
-x^2 - 2x + 11 + 4m = 0 \\
\\
\Delta = 4 + 4*(4m+11) = 4 + 16m +44  = 48 + 16m \\
\text{równanie ma 2 rozwiązania kiedy} \Delta = 0 \lor (\Delta > 0 \land x_{1}=-3) \\ \\
1) \ \ \ \ \ \Delta = 0 \\
48+16m = 0 \\
m = -3 \\
-x^2 - 2x + 11 + -12 = 0 \\
-x^2 - 2x -1 = 0 \\
-(x+1)^2 = 0 \\
x= -1 \\
2) \ \ \ \ \ \Delta > 0 \ \land \ x_{1} = -3 \\
m > -3 \\
-(-3)^2+6+11+4m = 0 \\
-9 + 6 +11 +4m = 0 \\
4m = -8 \\
m = -2 \in \{-3, + \infty \} \\
-x^2-2x+11-8 = 0  \\
-x^2-2x+3 = 0\\
\Delta = 4 + 12 = 16 \\
x = \frac{2 \pm 4}{-2} \\
x_{1} = -3 \notin D \\
x_{2} = 1
\end{gathered}
$$
### 1.78(interesting)
$$
\begin{gathered}
\frac{x+4a}{xa+a} - 2 = 0 \\
\frac{x+4a-2a(x+1)}{a(x+1)} = 0 \\
\frac{x+4a-2ax-2a}{a(x+1)} = 0 \\
\frac{x-2ax+2a}{a(x+1) } = 0 \\
\\
x \ne -1 \\
x-2ax = -2a \\ 
x(1-2a) = -2a \\
x = -\frac{2a}{1-2a}  = \frac{2a}{2a-1} \\ 
\\ \\
2a-1 \ne 0 \implies a \ne \frac{1}{2} \\
x \ne -1 \implies \frac{2a}{2a-1} \ne -1 \\
2a \ne-2a+1 \\ 
a \ne \frac{1}{4}
\\ \\ \\
a \in \mathbb{R} - \left\{ 0, \frac{1}{2}, \frac{1}{4} \right\}
\end{gathered}
$$
